Rework argument parsing, add --tight-bounds-mul-by
The `--tight-bounds-mul-by` argument allows us to specify the tight
bounds multiplier manually.

Closes #800
Closes #796 (actually, this had already been implemented, though we now
use it for curve25519)
Closes #755 (machine_wordsize is now owned by the binary as a whole)

Note that the last of these necessitates moving machine_wordsize to come
right after curve_description.  Invoking the binaries in the old way may
result in them hanging for a long time while they try to compute
representations for, say, lists of 2^255-19 5-bit-limbs for the "prime"
64.

We now use a structured language to describe the command line arguments,
based on OCaml's Arg module interface.  The error and help messages are
now perhaps a tiny bit worse, but it should now be moderately easier to
add new optional command line arguments.

Note that named arguments now use spaces rather than equals signs to
pass values.

The old usage message:
```
USAGE: ./src/ExtractionOCaml/unsaturated_solinas [--lang=LANGUAGE] [--static] [--internal-static] [--no-wide-int] [--widen-carry] [--widen-bytes] [--no-select] [--split-multiret] [--no-primitives] [--cmovznz-by-mul] curve_description n s-c machine_wordsize [function_to_synthesize*]
Got 0 arguments.

  LANGUAGE                The output language code should be emitted in.  Defaults to C if no language is given.  Case-sensitive.
                            Valid options are: C, Rust, Go, Java
  --static                Declare the functions as static, i.e., local to the file.
  --internal-static       Declare internal functions as static, i.e., local to the file.
  --no-wide-int           Don't use integers wider than the bitwidth.
  --widen-carry           Widen carry bit integer types to either the byte type, or to the full bitwidth if --widen-bytes is also passed.
  --widen-bytes           Widen byte types to the full bitwidth.
  --no-select             Use expressions that don't require cmov.
  --split-multiret        Don't allow instructions to return two results. This should always be set for bedrock2.
  --no-primitives         Suppress the generation of the bodies of primitive operations such as addcarryx, subborrowx, cmovznz, mulx, etc.
  --cmovznz-by-mul        Use an alternative implementation of cmovznz using multiplication rather than bitwise-and with -1.
  curve_description       A string which will be prefixed to every function name generated
  n                       The number of limbs, or the literal '(auto)' or '(autoN)' for a non-negative number N, to automatically guess the number of limbs
  s-c                     The prime, which must be expressed as a difference of a power of two and a small field element (e.g., '2^255 - 19', '2^448 - 2^224 - 1')
  machine_wordsize        The machine bitwidth (e.g., 32 or 64)
  function_to_synthesize  A space-separated list of functions that should be synthesized.  If no functions are given, all functions are synthesized.
                            Valid options are carry_mul, carry_square, carry, add, sub, opp, selectznz, to_bytes, from_bytes, or 'carry_scmul' followed by a decimal literal

Fatal error: exception Failure("Synthesis failed")
```

The new usage message:
```
./src/ExtractionOCaml/unsaturated_solinas: option 'curve_description' needs an argument.

USAGE: ./src/ExtractionOCaml/unsaturated_solinas [OPTS...] curve_description machine_wordsize n s-c [function_to_synthesize...]

  --lang {C|Rust|Go|Java}  The output language code should be emitted in.  Defaults to C if no language is given.  Case-sensitive.
  --static                 Declare the functions as static, i.e., local to the file.
  --internal-static        Declare internal functions as static, i.e., local to the file.
  --no-wide-int            Don't use integers wider than the bitwidth.
  --widen-carry            Widen carry bit integer types to either the byte type, or to the full bitwidth if --widen-bytes is also passed.
  --widen-bytes            Widen byte types to the full bitwidth.
  --no-select              Use expressions that don't require cmov.
  --split-multiret         Don't allow instructions to return two results. This should always be set for bedrock2.
  --no-primitives          Suppress the generation of the bodies of primitive operations such as addcarryx, subborrowx, cmovznz, mulx, etc.
  --cmovznz-by-mul         Use an alternative implementation of cmovznz using multiplication rather than bitwise-and with -1.
  --only-signed            Only allow signed integer types.
  --tight-bounds-mul-by    The (improper) fraction by which the (tight) bounds of each limb are scaled
  -h, --help               Display this list of options
  curve_description        A string which will be prefixed to every function name generated
  machine_wordsize         The machine bitwidth (e.g., 32 or 64)
  n                        The number of limbs, or the literal '(auto)' or '(autoN)' for a non-negative number N, to automatically guess the number of limbs
  s-c                      The prime, which must be expressed as a difference of a power of two and a small field element (e.g., '2^255 - 19', '2^448 - 2^224 - 1')
  function_to_synthesize   A space-separated list of functions that should be synthesized.  If no functions are given, all functions are synthesized.
                           Valid options are carry_mul, carry_square, carry, add, sub, opp, selectznz, to_bytes, from_bytes, or 'carry_scmul' followed by a decimal literal.

Fatal error: exception Failure("Synthesis failed")
```

src/CLI.v
@@ -23,6 +23,7 @@ Require Import Crypto.BoundsPipeline.
 Require Import Crypto.Stringification.Rust.
 Require Import Crypto.Stringification.Go.
 Require Import Crypto.Stringification.Java.
+Require Crypto.Util.Arg.
 Import ListNotations. Local Open Scope Z_scope. Local Open Scope string_scope.
 
 Import
@@ -30,6 +31,8 @@ Import
   Stringification.C.Compilers.
 
 Module ForExtraction.
+  Definition parse_string_and {T} (parse_T : string -> option T) (s : string) : option (string * T)
+    := option_map (@pair _ _ s) (parse_T s).
   Definition parse_Z (s : string) : option Z := parseZ_arith_strict s.
   Definition parse_N (s : string) : option N := parseN_arith_strict s.
   Definition parse_nat (s : string) : option nat := parsenat_arith_strict s.
@@ -140,7 +143,9 @@ Module ForExtraction.
 
   (** TODO: Write a better quoter and maybe move this elsewhere *)
   Definition quote (s : string) : string
-    := if List.existsb (fun ch => " " =? ch)%char (String.list_ascii_of_string s)
+    := if List.existsb (fun ch => List.existsb (fun badch => badch =? ch)%char
+                                               [" "; "("; ")"]%char)
+                       (String.list_ascii_of_string s)
        then "'" ++ s ++ "'"
        else s.
 
@@ -185,95 +190,111 @@ Module ForExtraction.
       languages list is used as the default. *)
   Definition default_supported_languages : supported_languagesT
     := [("C", ToString.OutputCAPI)
-       ; ("Rust", Rust.OutputRustAPI)
-       ; ("Go", Go.OutputGoAPI)
-       ; ("Java", Java.OutputJavaAPI)].
+        ; ("Rust", Rust.OutputRustAPI)
+        ; ("Go", Go.OutputGoAPI)
+        ; ("Java", Java.OutputJavaAPI)].
 
-  Definition curve_description_help
-    := "  curve_description       A string which will be prefixed to every function name generated".
-  Definition lang_help {supported_languages : supported_languagesT}
+  Local Notation anon_argT := (string * Arg.spec * Arg.doc)%type (only parsing).
+  Local Notation named_argT := (list Arg.key * Arg.spec * Arg.doc)%type (only parsing).
+
+  Definition curve_description_spec : anon_argT
+    := ("curve_description",
+        Arg.String,
+        ["A string which will be prefixed to every function name generated"]).
+  Definition lang_default {supported_languages : supported_languagesT}
+    := List.hd ("C", ToString.OutputCAPI) supported_languages.
+  Definition lang_spec {supported_languages : supported_languagesT} : named_argT
     := let supported_language_names := List.map (@fst _ _) supported_languages in
-       "  LANGUAGE                The output language code should be emitted in.  Defaults to " ++ List.hd "C" supported_language_names ++ " if no language is given.  Case-sensitive."
-         ++ String.NewLine ++
-       "                            Valid options are: " ++ String.concat ", " supported_language_names.
-  Definition total_help_indent
-    := "                          ".
-  Definition static_and_help
-    := ("--static", "Declare the functions as static, i.e., local to the file.").
-  Definition internal_static_and_help
-    := ("--internal-static", "Declare internal functions as static, i.e., local to the file.").
-  Definition only_signed_and_help
-    := ("--only-signed", "Only allow signed integer types.").
-  Definition no_select_and_help
-    := ("--no-select", "Use expressions that don't require cmov.").
-  Definition no_wide_int_and_help
-    := ("--no-wide-int", "Don't use integers wider than the bitwidth.").
-  Definition widen_carry_and_help
-    := ("--widen-carry", "Widen carry bit integer types to either the byte type, or to the full bitwidth if --widen-bytes is also passed.").
-  Definition widen_bytes_and_help
-    := ("--widen-bytes", "Widen byte types to the full bitwidth.").
-  Definition split_multiret_and_help
-    := ("--split-multiret", "Don't allow instructions to return two results. This should always be set for bedrock2.").
-  Definition no_primitives_and_help
-    := ("--no-primitives", "Suppress the generation of the bodies of primitive operations such as addcarryx, subborrowx, cmovznz, mulx, etc.").
-  Definition cmovznz_by_mul_and_help
-    := ("--cmovznz-by-mul", "Use an alternative implementation of cmovznz using multiplication rather than bitwise-and with -1.").
-  Definition n_help
-    := "  n                       The number of limbs, or the literal '(auto)' or '(autoN)' for a non-negative number N, to automatically guess the number of limbs".
-  Definition sc_help
-    := "  s-c                     The prime, which must be expressed as a difference of a power of two and a small field element (e.g., '2^255 - 19', '2^448 - 2^224 - 1')".
-  Definition m_help
-    := "  m                       The prime (e.g., '2^434 - (2^216*3^137 - 1)')".
-  Definition machine_wordsize_help
-    := "  machine_wordsize        The machine bitwidth (e.g., 32 or 64)".
-  Definition src_n_help
-    := "  src_n                   The number of limbs in the input".
-  Definition src_limbwidth_help
-    := "  src_limbwidth           The limbwidth of the input field element".
-  Definition dst_limbwidth_help
-    := "  dst_limbwidth           The limbwidth of the field element to be returned".
-  Definition use_bitwidth_in_and_help
-    := ("--use-bitwidth-in", "Instead of using an upper bound of s-1 on the input, use the maximum number that can be properly represented with the given base").
-  Definition use_bitwidth_out_and_help
-    := ("--use-bitwidth-out", "Instead of using an upper bound of s-1 on the output, use the maximum number that can be properly represented with the given base").
-  Definition inbounds_multiplier_help
-    := "  inbounds_multiplier     The (improper) fraction by which the bounds of each input limb are scaled (default: 1)".
-  Definition outbounds_multiplier_help
-    := "  outbounds_multiplier    The (improper) fraction by which the bounds of each output limb are scaled (default: 1)".
-  Definition inbounds_help
-    := "  inbounds                A semicolon-separated, square-bracked-surrounded list of integer expressions describing the input bounds.  Incompatible with --use-bitwidth-in.".
-  Definition outbounds_help
-    := "  outbounds               A semicolon-separated, square-bracked-surrounded list of integer expressions describing the output bounds.  Incompatible with --use-bitwidth-out.".
+       ([Arg.long_key "lang"],
+        Arg.CustomSymbol supported_languages,
+        ["The output language code should be emitted in.  Defaults to " ++ List.hd "C" supported_language_names ++ " if no language is given.  Case-sensitive."]).
+  Definition static_spec : named_argT
+    := ([Arg.long_key "static"], Arg.Unit, ["Declare the functions as static, i.e., local to the file."]).
+  Definition internal_static_spec : named_argT
+    := ([Arg.long_key "internal-static"], Arg.Unit, ["Declare internal functions as static, i.e., local to the file."]).
+  Definition only_signed_spec : named_argT
+    := ([Arg.long_key "only-signed"], Arg.Unit, ["Only allow signed integer types."]).
+  Definition no_select_spec : named_argT
+    := ([Arg.long_key "no-select"], Arg.Unit, ["Use expressions that don't require cmov."]).
+  Definition no_wide_int_spec : named_argT
+    := ([Arg.long_key "no-wide-int"], Arg.Unit, ["Don't use integers wider than the bitwidth."]).
+  Definition widen_carry_spec : named_argT
+    := ([Arg.long_key "widen-carry"], Arg.Unit, ["Widen carry bit integer types to either the byte type, or to the full bitwidth if --widen-bytes is also passed."]).
+  Definition widen_bytes_spec : named_argT
+    := ([Arg.long_key "widen-bytes"], Arg.Unit, ["Widen byte types to the full bitwidth."]).
+  Definition split_multiret_spec : named_argT
+    := ([Arg.long_key "split-multiret"], Arg.Unit, ["Don't allow instructions to return two results. This should always be set for bedrock2."]).
+  Definition no_primitives_spec : named_argT
+    := ([Arg.long_key "no-primitives"], Arg.Unit, ["Suppress the generation of the bodies of primitive operations such as addcarryx, subborrowx, cmovznz, mulx, etc."]).
+  Definition cmovznz_by_mul_spec : named_argT
+    := ([Arg.long_key "cmovznz-by-mul"], Arg.Unit, ["Use an alternative implementation of cmovznz using multiplication rather than bitwise-and with -1."]).
+  Definition tight_bounds_multiplier_default := default_tight_upperbound_fraction.
+  Definition tight_bounds_multiplier_spec : named_argT
+    := ([Arg.long_key "tight-bounds-mul-by"],
+        Arg.Custom (parse_string_and parse_Q) "ℚ",
+        ["The (improper) fraction by which the (tight) bounds of each limb are scaled"]).
+  Definition n_spec : anon_argT
+    := ("n",
+        Arg.Custom (parse_string_and parse_n) "an ℕ or the literal '(auto)' or '(autoN)' for a non-negative number N",
+        ["The number of limbs, or the literal '(auto)' or '(autoN)' for a non-negative number N, to automatically guess the number of limbs"]).
+  Definition sc_spec : anon_argT
+    := ("s-c",
+        Arg.Custom (parse_string_and parse_sc) "an integer expression",
+        ["The prime, which must be expressed as a difference of a power of two and a small field element (e.g., '2^255 - 19', '2^448 - 2^224 - 1')"]).
+  Definition m_spec : anon_argT
+    := ("m",
+        Arg.Custom (parse_string_and parse_m) "an integer expression",
+        ["The prime (e.g., '2^434 - (2^216*3^137 - 1)')"]).
+  Definition machine_wordsize_spec : anon_argT
+    := ("machine_wordsize",
+        Arg.Custom (parse_string_and parse_machine_wordsize) "an integer",
+        ["The machine bitwidth (e.g., 32 or 64)"]).
+  Definition src_n_spec : anon_argT
+    := ("src_n",
+        Arg.Custom (parse_string_and parse_src_n) "ℕ",
+        ["The number of limbs in the input"]).
+  Definition src_limbwidth_spec : anon_argT
+    := ("src_limbwidth",
+        Arg.Custom (parse_string_and parse_limbwidth) "ℕ",
+        ["The limbwidth of the input field element"]).
+  Definition dst_limbwidth_spec : anon_argT
+    := ("dst_limbwidth",
+        Arg.Custom (parse_string_and parse_limbwidth) "ℕ",
+        ["The limbwidth of the field element to be returned"]).
+  Definition use_bitwidth_in_spec : named_argT
+    := ([Arg.long_key "use-bitwidth-in"],
+        Arg.Unit,
+        ["Instead of using an upper bound of s-1 on the input, use the maximum number that can be properly represented with the given base"]).
+  Definition use_bitwidth_out_spec : named_argT
+    := ([Arg.long_key "use-bitwidth-out"],
+        Arg.Unit,
+        ["Instead of using an upper bound of s-1 on the output, use the maximum number that can be properly represented with the given base"]).
+  Definition default_inbounds_multiplier := 1.
+  Definition inbounds_multiplier_spec : named_argT
+    := ([Arg.long_key "inbounds-multiplier"],
+        Arg.String,
+        ["The (improper) fraction by which the bounds of each input limb are scaled (default: " ++ show false default_inbounds_multiplier ++ ")"]).
+  Definition default_outbounds_multiplier := 1.
+  Definition outbounds_multiplier_spec : named_argT
+    := ([Arg.long_key "outbounds-multiplier"],
+        Arg.String,
+        ["The (improper) fraction by which the bounds of each output limb are scaled (default: " ++ show false default_outbounds_multiplier ++ ")"]).
+  Definition inbounds_spec : named_argT
+    := ([Arg.long_key "inbounds"],
+        Arg.String,
+        ["A semicolon-separated, square-bracked-surrounded list of integer expressions describing the input bounds.  Incompatible with --use-bitwidth-in."]).
+  Definition outbounds_spec : named_argT
+    := ([Arg.long_key "outbounds"],
+        Arg.String,
+        ["A semicolon-separated, square-bracked-surrounded list of integer expressions describing the output bounds.  Incompatible with --use-bitwidth-out."]).
+  Definition function_to_synthesize_spec (valid_names : string) : anon_argT
+    := ("function_to_synthesize",
+        Arg.String,
+        ["A space-separated list of functions that should be synthesized.  If no functions are given, all functions are synthesized."
+         ; "Valid options are " ++ valid_names ++ "."]).
 
-  Definition function_to_synthesize_help (valid_names : string)
-    := "  function_to_synthesize  A space-separated list of functions that should be synthesized.  If no functions are given, all functions are synthesized."
-         ++ String.NewLine ++
-         "                            Valid options are " ++ valid_names.
-
-  Definition common_optional_options
-    := [static_and_help
-        ; internal_static_and_help
-        ; no_wide_int_and_help
-        ; widen_carry_and_help
-        ; widen_bytes_and_help
-        ; no_select_and_help
-        ; split_multiret_and_help
-        ; no_primitives_and_help
-        ; cmovznz_by_mul_and_help
-       ].
-  Definition optional_options_to_usage {T} opt_options
-    := String.concat " " (List.map (fun '((opt, _) : _ * T) => "[" ++ opt ++ "]") opt_options).
-  Definition common_usage_opts := optional_options_to_usage common_optional_options.
-
-  Definition to_help (s : string * string)
-    := let opt := "  " ++ fst s in
-       let descr := snd s in
-       opt ++ String.substring 0 (String.length total_help_indent - String.length opt) total_help_indent ++ descr.
-
-
-  Local Set Primitive Projections.
-  Record > Dyn := dyn { dyn_ty : Type ; dyn_val :> option dyn_ty }.
-  Arguments dyn {_} _.
+  Definition collapse_list_default {A} (default : A) (ls : list A)
+    := List.hd default (List.rev ls).
 
   Definition join_errors {A B} (x : A + list string) (y : B + list string) : (A * B) + list string
     := match x, y with
@@ -281,85 +302,6 @@ Module ForExtraction.
        | inr err, inl _ | inl _, inr err => inr err
        | inl x, inl y => inl (x, y)
        end.
-
-  Fixpoint parse_resultL' (acc : Type) (ls : list (string (* name *) * string (* string value *) * Dyn))
-    : Type
-    := match ls with
-       | nil => acc
-       | cons (_, _, {| dyn_ty := T |}) ls'
-         => parse_resultL' (acc * T) ls'
-       end.
-  Definition parse_resultL (ls : list (string (* name *) * string (* string value *) * Dyn))
-    := match ls return Type with
-       | nil => unit
-       | cons (_, _, {| dyn_ty := T |}) ls'
-         => parse_resultL' T ls' + list string
-       end%type.
-
-  Fixpoint parse_many' {accT : Type} (acc : accT)
-           (ls : list (string (* name *) * string (* string value *) * Dyn))
-    : parse_resultL' accT ls + list string
-    := match ls return parse_resultL' accT ls + list string with
-       | nil => inl acc
-       | cons (_, _, {| dyn_val := Some v |}) ls'
-         => @parse_many' _ (acc, v) ls'
-       | cons (name, str_val, {| dyn_val := None |}) ls'
-         => let err_ls := match @parse_many' _ tt ls' with
-                          | inl _ => nil
-                          | inr err_ls => err_ls
-                          end in
-            inr ((name ++ " (" ++ str_val ++ ")")%string :: err_ls)
-       end.
-
-  Definition parse_many
-             (ls : list (string (* name *) * string (* string value *) * Dyn))
-    : parse_resultL ls
-    := let transform_err T (v : T + list string)
-           := match v with
-              | inl v => inl v
-              | inr nil => inr ["Internal Error: Parse failure without an error message"]
-              | inr ls => inr ["Could not parse " ++ String.concat " nor " ls]
-              end%string in
-       match ls with
-       | nil => tt
-       | cons (_, _, {| dyn_val := Some v |}) ls'
-         => transform_err _ (@parse_many' _ v ls')
-       | cons (name, str_val, {| dyn_val := None |}) ls'
-         => let err_ls := match @parse_many' _ tt ls' with
-                          | inl _ => nil
-                          | inr err_ls => err_ls
-                          end in
-            transform_err _ (inr ((name ++ " (" ++ str_val ++ ")")%string :: err_ls))
-       end.
-
-  (** if [opt] is in [tl argv], remove all instances of it, and return
-      [(filter-out opt argv, true)]; otherwise, return [(argv, false)]
-      *)
-  Definition argv_to_contains_opt_and_argv (opt : string) (argv : list string)
-    : list string * bool
-    := match argv with
-       | prog_name :: rest
-         => let is_opt arg := (arg =? opt)%string in
-            (prog_name :: filter (fun arg => negb (is_opt arg)) rest,
-             existsb is_opt rest)
-       | _ => (argv, false)
-       end.
-
-  (** return the remainder of all elements of [argv] starting with
-      [opt], and all elements which do not start with [opt] *)
-  Definition argv_to_startswith_opt_and_argv (opt : string) (argv : list string)
-    := let '(opts, argv) := List.partition (String.contains 0 opt) argv in
-       (argv,
-        List.map (fun s => String.substring (String.length opt) (String.length s) s) opts).
-
-  Definition argv_to_single_startswith_opt_and_argv (opt : string) (argv : list string)
-    := let '(argv, opts) := argv_to_startswith_opt_and_argv opt argv in
-       (argv,
-        match opts with
-        | [] => inl None
-        | [opt] => inl (Some opt)
-        | _ => inr opts
-        end).
 
   (** We define a class for holding the various options we might pass to [Synthesize] *)
   Class SynthesizeOptions :=
@@ -391,36 +333,75 @@ Module ForExtraction.
       ; machine_wordsize :> machine_wordsize_opt
     }.
 
+  Definition common_optional_options {supported_languages : supported_languagesT}
+    := [lang_spec
+        ; static_spec
+        ; internal_static_spec
+        ; no_wide_int_spec
+        ; widen_carry_spec
+        ; widen_bytes_spec
+        ; no_select_spec
+        ; split_multiret_spec
+        ; no_primitives_spec
+        ; cmovznz_by_mul_spec
+        ; only_signed_spec
+       ].
+
+  Definition parse_common_optional_options
+             {supported_languages : supported_languagesT}
+             {machine_wordsizev : machine_wordsize_opt}
+             (data : Arg.keyed_spec_list_data common_optional_options)
+    : (SynthesizeOptions * ToString.OutputLanguageAPI) + list string
+    := let '(langv
+             , staticv
+             , internal_staticv
+             , no_wide_intv
+             , widen_carryv
+             , widen_bytesv
+             , no_selectv
+             , split_multiretv
+             , no_primitivesv
+             , cmovznz_by_mulv
+             , only_signedv
+            ) := data in
+       let to_bool ls := (0 <? List.length ls)%nat in
+       let res
+           := ({| static := to_bool staticv
+                  ; internal_static := to_bool internal_staticv
+                  ; widen_carry := to_bool widen_carryv
+                  ; widen_bytes := to_bool widen_bytesv
+                  ; no_select := to_bool no_selectv
+                  ; only_signed := to_bool only_signedv
+                  ; should_split_mul := to_bool no_wide_intv
+                  ; should_split_multiret := to_bool split_multiretv
+                  ; use_mul_for_cmovznz := to_bool cmovznz_by_mulv
+                  ; emit_primitives := negb (to_bool no_primitivesv)
+               |},
+               snd (List.hd lang_default langv)) in
+       match langv with
+       | [] | [_] => inl res
+       | opts => inr ["Only one language specification with --lang is allowed; multiple languages were requested: " ++ String.concat ", " (List.map (@fst _ _) opts)]
+       end.
+
   (** We define a class for the various operations that are specific to a pipeline *)
   Class PipelineAPI :=
     {
-      (** The type of special arguments that all pipelines need access to *)
-      SpecialParsedArgsT : Type
-      := machine_wordsize_opt;
+      (** The spec of curve-specific command line arguments *)
+      spec : Arg.arg_spec;
       (** Type of arguments parsed from the command line *)
       ParsedArgsT : Type;
       (** Type of (unparsed) arguments remembered from the command line *)
       StringArgsT : Type;
       ArgsT := (StringArgsT * ParsedArgsT)%type;
 
-      (** Takes in argv except without the binary name and without any
-          general options (such as language), and parses the
-          curve-specific arguments, returning either [Some (inl
-          value)], [Some (inr errors)], or [None] if there are not
-          enough arguments and the usage string should be displayed. *)
-      parse_args : list string -> option (ArgsT + list string);
-
-      (** Takes in parsed args and computes common arguments *)
-      extract_known_args : ParsedArgsT -> SpecialParsedArgsT;
+      (** Takes in args parsed via the spec and post-parses
+          curve-specific arguments, returning either [inl value] or
+          [inr errors] *)
+      parse_args : forall {synthesize_opts : SynthesizeOptions}, Arg.arg_spec_results spec -> ArgsT + list string;
 
       (** Renders a header at the top displaying the command line
           arguments.  Will be wrapped in a comment block *)
       show_lines_args : ArgsT -> list string;
-
-      (** The part of the usage-string for arguments after curve_description *)
-      pipeline_usage_string : string;
-      (** The list of help strings (to be joined by newlines) *)
-      help_lines : list string;
 
       (** The Synthesize function from the pipeline *)
       (** N.B. [comment_header] will be passed in *without* wrapping
@@ -445,12 +426,14 @@ Module ForExtraction.
                  {synthesize_opts : SynthesizeOptions}
                  (invocation : string)
                  (curve_description : string)
+                 (str_machine_wordsize : string)
                  (args : ArgsT)
         : list (string * Pipeline.ErrorT (list string)) + list string
         := let prefix := ("fiat_" ++ curve_description ++ "_")%string in
            let header :=
-               ((["Autogenerated: " ++ invocation;
-                    "curve description: " ++ curve_description]%string)
+               ((["Autogenerated: " ++ invocation
+                  ; "curve description: " ++ curve_description
+                  ; "machine_wordsize = " ++ show false (machine_wordsize:Z) ++ " (from """ ++ str_machine_wordsize ++ """)"]%string)
                   ++ show_lines_args args)%list in
            inl (Synthesize (snd args) header prefix).
 
@@ -462,9 +445,10 @@ Module ForExtraction.
                  {synthesize_opts : SynthesizeOptions}
                  (invocation : string)
                  (curve_description : string)
+                 (str_machine_wordsize : string)
                  (args : ArgsT)
         : list string + list string
-        := match CollectErrors (PipelineLines invocation curve_description args) with
+        := match CollectErrors (PipelineLines invocation curve_description str_machine_wordsize args) with
            | inl ls
              => inl
                   (List.map (fun s => String.concat String.NewLine (List.map strip_trailing_spaces s) ++ String.NewLine ++ String.NewLine)
@@ -482,33 +466,15 @@ Module ForExtraction.
                  {synthesize_opts : SynthesizeOptions}
                  (invocation : string)
                  (curve_description : string)
+                 (str_machine_wordsize : string)
                  (args : ArgsT)
                  (success : list string -> A)
                  (error : list string -> A)
         : A
-        := match ProcessedLines invocation curve_description args with
+        := match ProcessedLines invocation curve_description str_machine_wordsize args with
            | inl s => success s
            | inr s => error s
            end.
-
-      Definition argv_to_language_and_argv
-                 {supported_languages : supported_languagesT}
-                 (argv : list string)
-        : list string * (ToString.OutputLanguageAPI + list string)
-        := let '(argv, opts) := argv_to_startswith_opt_and_argv "--lang=" argv in
-           (argv,
-            match opts with
-            | [] => inl (* if no is --lang=<something known>, default to the first element of the list, or else C if supported languages are empty *)
-                      (List.hd ToString.OutputCAPI (List.map (@snd _ _) supported_languages))
-            | [lang]
-              => match List.filter (fun '(known_lang, _) => String.eqb lang known_lang) supported_languages with
-                 | [] => inr ["Unknown language " ++ lang ++ " requested; supported languages are " ++ String.concat ", " (List.map (@fst _ _) supported_languages)]
-                 | [(_, output_api)] => inl output_api
-                 | _ => inr ["Internal Error: Multiple languages exist with the same name (" ++ lang ++ ")"]
-                 end
-            | _
-              => inr ["Only one language specification with --lang is allowed; multiple languages were requested: " ++ String.concat ", " opts]
-            end).
 
       Definition PipelineMain
                  {supported_languages : supported_languagesT}
@@ -518,59 +484,26 @@ Module ForExtraction.
                  (error : list string -> A)
         : A
         := let invocation := String.concat " " (List.map quote argv) in
-           let on_wrong_argv _ :=
-               match argv with
-               | nil => error ["empty argv"]
-               | prog::args
-                 => error ((["USAGE: " ++ prog ++ " [--lang=LANGUAGE] " ++ common_usage_opts ++ " curve_description " ++ pipeline_usage_string;
-                               "Got " ++ show false (List.length args) ++ " arguments.";
-                               "";
-                               lang_help]%string)
-                             ++ List.map to_help common_optional_options
-                             ++ [curve_description_help]
-                             ++ help_lines
-                             ++ [""])%list
-               end in
-           let '(argv, output_language_api) := argv_to_language_and_argv argv in
-           let '(argv, staticv) := argv_to_contains_opt_and_argv "--static" argv in
-           let '(argv, internal_staticv) := argv_to_contains_opt_and_argv "--internal-static" argv in
-           let '(argv, only_signedv) := argv_to_contains_opt_and_argv "--only-signed" argv in
-           let '(argv, no_selectv) := argv_to_contains_opt_and_argv "--no-select" argv in
-           let '(argv, no_wide_intsv) := argv_to_contains_opt_and_argv "--no-wide-int" argv in
-           let '(argv, use_mul_for_cmovznzv) := argv_to_contains_opt_and_argv "--cmovznz-by-mul" argv in
-           let '(argv, widen_carryv) := argv_to_contains_opt_and_argv "--widen-carry" argv in
-           let '(argv, widen_bytesv) := argv_to_contains_opt_and_argv "--widen-bytes" argv in
-           let '(argv, split_multiretv) := argv_to_contains_opt_and_argv "--split-multiret" argv in
-           let '(argv, no_primitivesv) := argv_to_contains_opt_and_argv "--no-primitives" argv in
-           (** must come last *)
-           let '(argv, unrecognized_args) := argv_to_startswith_opt_and_argv "--" argv in
-           match List.map (fun s => "Unrecognized argument: --" ++ s)%string unrecognized_args,
-                 output_language_api,
-                 argv with
-           | nil, inl output_language_api, _::curve_description::args
-             => match parse_args args with
-                | Some (inl args)
-                  => let machine_wordsizev := extract_known_args (snd args) in
-                     let opts
-                         := {| static := staticv
-                               ; internal_static := internal_staticv
-                               ; only_signed := only_signedv
-                               ; no_select := no_selectv
-                               ; use_mul_for_cmovznz := use_mul_for_cmovznzv
-                               ; widen_carry := widen_carryv
-                               ; widen_bytes := widen_bytesv
-                               ; should_split_mul := no_wide_intsv
-                               ; should_split_multiret := split_multiretv
-                               ; emit_primitives := negb no_primitivesv
-                               ; machine_wordsize := machine_wordsizev |} in
-                     Pipeline invocation curve_description args success error
-                | Some (inr errs)
-                  => error errs
-                | None => on_wrong_argv tt
+           let full_spec
+               := {| Arg.named_args := common_optional_options ++ spec.(Arg.named_args)
+                     ; Arg.anon_args := curve_description_spec :: machine_wordsize_spec :: spec.(Arg.anon_args)
+                     ; Arg.anon_opt_args := spec.(Arg.anon_opt_args)
+                     ; Arg.anon_opt_repeated_arg := spec.(Arg.anon_opt_repeated_arg) |} in
+           match Arg.parse_argv argv full_spec with
+           | ErrorT.Success (named_data, anon_data, anon_opt_data, anon_opt_repeated_data)
+             => let '(common_named_data, named_data) := Arg.split_type_of_list' (ls1:=List.map _ common_optional_options) named_data in
+                let '((curve_description, (str_machine_wordsize, machine_wordsize)), anon_data) := Arg.split_type_of_list' (ls1:=[_;_]) anon_data in
+                let machine_wordsize : machine_wordsize_opt := machine_wordsize in
+                match parse_common_optional_options common_named_data with
+                | inl (opts, output_language_api)
+                  => match parse_args (named_data, anon_data, anon_opt_data, anon_opt_repeated_data) with
+                     | inl args
+                       => Pipeline invocation curve_description str_machine_wordsize args success error
+                     | inr errs => error errs
+                     end
+                | inr errs => error errs
                 end
-           | nil, inl _, _ => on_wrong_argv tt
-           | unrecognized_args_errs, inr errs, _ => error (errs ++ unrecognized_args_errs)%list
-           | unrecognized_args_errs, inl _, _ => error unrecognized_args_errs
+           | ErrorT.Error err => error (Arg.show_list_parse_error full_spec err)
            end.
     End __.
   End Parameterized.
@@ -578,53 +511,37 @@ Module ForExtraction.
   Module UnsaturatedSolinas.
     Local Instance api : PipelineAPI
       := {
-          parse_args (args : list string)
-          := match args with
-             | n::sc::machine_wordsize::requests
-               => let str_n := n in
-                  let str_machine_wordsize := machine_wordsize in
-                  let str_sc := sc in
-                  let show_requests := match requests with nil => "(all)" | _ => String.concat ", " requests end in
-                  Some
-                    match parse_many [("n", n, parse_n n:Dyn)
-                                      ; ("machine_wordsize", machine_wordsize, parse_machine_wordsize machine_wordsize:Dyn)
-                                      ; ("s-c", sc, parse_sc sc:Dyn)] with
-                    | inr errs => inr errs
-                    | inl (n, machine_wordsize, (s, c))
-                      => match get_num_limbs s c machine_wordsize n, n with
-                         | None, NumLimbs n => inr ["Internal error: get_num_limbs (on (" ++ PowersOfTwo.show_Z false s ++ ", " ++ show_c false c ++ ", " ++ show false machine_wordsize ++ ", " ++ show false n ++ ")) returned None even though the argument was NumLimbs"]
-                         | None, Auto idx => inr ["Invalid index " ++ show false idx ++ " when guessing the number of limbs for s-c = " ++ PowersOfTwo.show_Z false s ++ " - " ++ show_c false c ++ "; valid indices must index into the list " ++ show false (get_possible_limbs s c machine_wordsize) ++ "."]
-                         | Some n, _
-                           => inl
-                                ((str_n, str_machine_wordsize, str_sc, show_requests),
-                                 (n, machine_wordsize, s, c, requests))
-                         end
-                    end
-             | _ => None
+          spec :=
+            {| Arg.named_args := [tight_bounds_multiplier_spec]
+               ; Arg.anon_args := [n_spec; sc_spec]
+               ; Arg.anon_opt_args := []
+               ; Arg.anon_opt_repeated_arg := Some (function_to_synthesize_spec UnsaturatedSolinas.valid_names) |};
+
+          parse_args opts args
+          := let '(tight_bounds_multiplier, ((str_n, n), (str_sc, (s, c))), tt, requests) := args in
+             let show_requests := match requests with nil => "(all)" | _ => String.concat ", " requests end in
+             let '(str_tight_bounds_multiplier, tight_bounds_multiplier) := collapse_list_default ("", tight_bounds_multiplier_default) (List.map (@snd _ _) tight_bounds_multiplier) in
+             let tight_bounds_multiplier : tight_upperbound_fraction_opt := tight_bounds_multiplier in
+             match get_num_limbs s c machine_wordsize n, n with
+             | None, NumLimbs n => inr ["Internal error: get_num_limbs (on (" ++ PowersOfTwo.show_Z false s ++ ", " ++ show_c false c ++ ", " ++ show false (machine_wordsize:Z) ++ ", " ++ show false n ++ ")) returned None even though the argument was NumLimbs"]
+             | None, Auto idx => inr ["Invalid index " ++ show false idx ++ " when guessing the number of limbs for s-c = " ++ PowersOfTwo.show_Z false s ++ " - " ++ show_c false c ++ "; valid indices must index into the list " ++ show false (get_possible_limbs s c machine_wordsize) ++ "."]
+             | Some n, _
+               => inl
+                    ((str_n, str_sc, str_tight_bounds_multiplier, show_requests),
+                     (n, s, c, tight_bounds_multiplier, requests))
              end;
 
-          extract_known_args :=
-            fun '(n, machine_wordsize, s, c, requests)
-            => machine_wordsize;
-
           show_lines_args :=
-            fun '((str_n, str_machine_wordsize, str_sc, show_requests),
-                  (n, machine_wordsize, s, c, requests))
+            fun '((str_n, str_sc, str_tight_bounds_multiplier, show_requests),
+                  (n, s, c, tight_bounds_multiplier, requests))
             => ["requested operations: " ++ show_requests;
-                  "n = " ++ show false n ++ " (from """ ++ str_n ++ """)";
-                  "s-c = " ++ PowersOfTwo.show_Z false s ++ " - " ++ show_c false c ++ " (from """ ++ str_sc ++ """)";
-                  "machine_wordsize = " ++ show false machine_wordsize ++ " (from """ ++ str_machine_wordsize ++ """)"]%string;
-
-          pipeline_usage_string := "n s-c machine_wordsize [function_to_synthesize*]";
-
-          help_lines := [n_help;
-                           sc_help;
-                           machine_wordsize_help;
-                           function_to_synthesize_help UnsaturatedSolinas.valid_names];
+               "n = " ++ show false n ++ " (from """ ++ str_n ++ """)";
+               "s-c = " ++ PowersOfTwo.show_Z false s ++ " - " ++ show_c false c ++ " (from """ ++ str_sc ++ """)";
+               "tight_bounds_multiplier = " ++ show false (tight_bounds_multiplier:Q) ++ " (from """ ++ str_tight_bounds_multiplier ++ """)"]%string;
 
           Synthesize
-          := fun _ opts '(n, machine_wordsize, s, c, requests) comment_header prefix
-             => UnsaturatedSolinas.Synthesize n s c machine_wordsize comment_header prefix requests
+          := fun _ opts '(n, s, c, tight_bounds_multiplier, requests) comment_header prefix
+             => UnsaturatedSolinas.Synthesize n s c machine_wordsize comment_header prefix requests;
         }.
 
     Definition PipelineMain
@@ -640,49 +557,33 @@ Module ForExtraction.
   Module WordByWordMontgomery.
     Local Instance api : PipelineAPI
       := {
-          parse_args (args : list string)
-          := match args with
-             | m::machine_wordsize::requests
-               => let str_machine_wordsize := machine_wordsize in
-                  let str_m := m in
-                  let show_requests := match requests with nil => "(all)" | _ => String.concat ", " requests end in
-                  Some
-                    match parse_many [("machine_wordsize", machine_wordsize, parse_machine_wordsize machine_wordsize:Dyn);
-                                        ("m", m, parse_m m:Dyn)] with
-                    | inr errs => inr errs
-                    | inl (machine_wordsize, m)
-                      => inl ((str_machine_wordsize, str_m, show_requests),
-                              (machine_wordsize, m, requests))
-                    end
-             | _ => None
-             end;
+          spec :=
+            {| Arg.named_args := []
+               ; Arg.anon_args := [m_spec]
+               ; Arg.anon_opt_args := []
+               ; Arg.anon_opt_repeated_arg := Some (function_to_synthesize_spec WordByWordMontgomery.valid_names) |};
 
-          extract_known_args :=
-            fun '(machine_wordsize, m, requests)
-            => machine_wordsize;
+          parse_args opts args
+          := let '(tt, (str_m, m), tt, requests) := args in
+             let show_requests := match requests with nil => "(all)" | _ => String.concat ", " requests end in
+             inl ((str_m, show_requests),
+                  (m, requests));
 
           show_lines_args :=
-            fun '((str_machine_wordsize, str_m, show_requests),
-                  (machine_wordsize, m, requests))
+            fun '((str_m, show_requests),
+                  (m, requests))
             => ["requested operations: " ++ show_requests;
-                  "m = " ++ Hex.show_Z false m ++ " (from """ ++ str_m ++ """)";
-                  "machine_wordsize = " ++ show false machine_wordsize ++ " (from """ ++ str_machine_wordsize ++ """)";
-                  "                                                                  ";
-                  "NOTE: In addition to the bounds specified above each function, all";
-                  "  functions synthesized for this Montgomery arithmetic require the";
-                  "  input to be strictly less than the prime modulus (m), and also  ";
-                  "  require the input to be in the unique saturated representation. ";
-                  "  All functions also ensure that these two properties are true of ";
-                  "  return values.                                                  "];
-
-          pipeline_usage_string := "m machine_wordsize [function_to_synthesize*]";
-
-          help_lines := [m_help;
-                           machine_wordsize_help;
-                           function_to_synthesize_help WordByWordMontgomery.valid_names];
+               "m = " ++ Hex.show_Z false m ++ " (from """ ++ str_m ++ """)";
+               "                                                                  ";
+               "NOTE: In addition to the bounds specified above each function, all";
+               "  functions synthesized for this Montgomery arithmetic require the";
+               "  input to be strictly less than the prime modulus (m), and also  ";
+               "  require the input to be in the unique saturated representation. ";
+               "  All functions also ensure that these two properties are true of ";
+               "  return values.                                                  "];
 
           Synthesize
-          := fun _ opts '(machine_wordsize, m, requests) comment_header prefix
+          := fun _ opts '(m, requests) comment_header prefix
              => WordByWordMontgomery.Synthesize m machine_wordsize comment_header prefix requests
         }.
 
@@ -699,42 +600,26 @@ Module ForExtraction.
   Module SaturatedSolinas.
     Local Instance api : PipelineAPI
       := {
-          parse_args (args : list string)
-          := match args with
-             | sc::machine_wordsize::requests
-               => let str_machine_wordsize := machine_wordsize in
-                  let str_sc := sc in
-                  let show_requests := match requests with nil => "(all)" | _ => String.concat ", " requests end in
-                  Some
-                    match parse_many [("machine_wordsize", machine_wordsize, parse_machine_wordsize machine_wordsize:Dyn)
-                                      ; ("s-c", sc, parse_sc sc:Dyn)] with
-                    | inr errs => inr errs
-                    | inl (machine_wordsize, (s, c))
-                      => inl ((str_machine_wordsize, str_sc, show_requests),
-                              (machine_wordsize, s, c, requests))
-                    end
-             | _ => None
-             end;
+          spec :=
+            {| Arg.named_args := []
+               ; Arg.anon_args := [sc_spec]
+               ; Arg.anon_opt_args := []
+               ; Arg.anon_opt_repeated_arg := Some (function_to_synthesize_spec SaturatedSolinas.valid_names) |};
 
-          extract_known_args :=
-            fun '(machine_wordsize, s, c, requests)
-            => machine_wordsize;
+          parse_args opts args
+          := let '(tt, (str_sc, (s, c)), tt, requests) := args in
+             let show_requests := match requests with nil => "(all)" | _ => String.concat ", " requests end in
+             inl ((str_sc, show_requests),
+                  (s, c, requests));
 
           show_lines_args :=
-            fun '((str_machine_wordsize, str_sc, show_requests),
-                  (machine_wordsize, s, c, requests))
+            fun '((str_sc, show_requests),
+                  (s, c, requests))
             => ["requested operations: " ++ show_requests;
-                  "s-c = " ++ PowersOfTwo.show_Z false s ++ " - " ++ show_c false c ++ " (from """ ++ str_sc ++ """)";
-                  "machine_wordsize = " ++ show false machine_wordsize ++ " (from """ ++ str_machine_wordsize ++ """)"];
-
-          pipeline_usage_string := "s-c machine_wordsize [function_to_synthesize*]";
-
-          help_lines := [sc_help;
-                           machine_wordsize_help;
-                           function_to_synthesize_help SaturatedSolinas.valid_names];
+               "s-c = " ++ PowersOfTwo.show_Z false s ++ " - " ++ show_c false c ++ " (from """ ++ str_sc ++ """)"];
 
           Synthesize
-          := fun _ opts '(machine_wordsize, s, c, requests) comment_header prefix
+          := fun _ opts '(s, c, requests) comment_header prefix
              => SaturatedSolinas.Synthesize s c machine_wordsize comment_header prefix requests
         }.
 
@@ -751,82 +636,59 @@ Module ForExtraction.
   Module BaseConversion.
     Local Instance api : PipelineAPI
       := {
-          parse_args (args : list string)
-          := let '(args, inbounds_multiplier) := argv_to_single_startswith_opt_and_argv "--inbounds-multiplier=" args in
-             let '(args, outbounds_multiplier) := argv_to_single_startswith_opt_and_argv "--outbounds-multiplier=" args in
-             let '(args, inbounds) := argv_to_single_startswith_opt_and_argv "--inbounds=" args in
-             let '(args, outbounds) := argv_to_single_startswith_opt_and_argv "--outbounds=" args in
-             let '(args, use_bitwidth_in) := argv_to_contains_opt_and_argv "--use-bitwidth-in" args in
-             let '(args, use_bitwidth_out) := argv_to_contains_opt_and_argv "--use-bitwidth-out" args in
-             let '(str_inbounds_multiplier, inbounds_multiplier) := parse_dirbounds_multiplier "in" inbounds_multiplier in
-             let '(str_outbounds_multiplier, outbounds_multiplier) := parse_dirbounds_multiplier "out" outbounds_multiplier in
-             let '(str_inbounds, inbounds) := parse_dirbounds "in" inbounds use_bitwidth_in in
-             let '(str_outbounds, outbounds) := parse_dirbounds "out" outbounds use_bitwidth_out in
-             match args with
-             | src_n::sc::src_limbwidth::dst_limbwidth::machine_wordsize::requests
-               => let str_src_n := src_n in
-                  let str_sc := sc in
-                  let str_src_limbwidth := src_limbwidth in
-                  let str_dst_limbwidth := dst_limbwidth in
-                  let str_machine_wordsize := machine_wordsize in
-                  let show_requests := match requests with nil => "(all)" | _ => String.concat ", " requests end in
-                  Some
-                    match join_errors
-                            (parse_many [("src_n", src_n, parse_src_n src_n:Dyn)
-                                         ; ("s-c", sc, parse_sc sc:Dyn)
-                                         ; ("src_limbwidth", src_limbwidth, parse_limbwidth src_limbwidth:Dyn)
-                                         ; ("dst_limbwidth", dst_limbwidth, parse_limbwidth dst_limbwidth:Dyn)
-                                         ; ("machine_wordsize", machine_wordsize, parse_machine_wordsize machine_wordsize:Dyn)])
-                            (join_errors
-                               (join_errors
-                                  inbounds_multiplier
-                                  outbounds_multiplier)
-                               (join_errors
-                                  inbounds
-                                  outbounds))
-                    with
-                    | inr errs => inr errs
-                    | inl ((src_n, (s, c), src_limbwidth, dst_limbwidth, machine_wordsize), ((inbounds_multiplier, outbounds_multiplier), (inbounds, outbounds)))
-                      => inl ((str_src_n, str_sc, str_src_limbwidth, str_dst_limbwidth, str_machine_wordsize, str_inbounds_multiplier, str_outbounds_multiplier, use_bitwidth_in, use_bitwidth_out, str_inbounds, str_outbounds, show_requests),
-                              (src_n, s, c, src_limbwidth, dst_limbwidth, machine_wordsize, inbounds_multiplier, outbounds_multiplier, inbounds, outbounds, requests))
-                    end
-             | _ => None
+          spec :=
+            {| Arg.named_args := [inbounds_multiplier_spec; outbounds_multiplier_spec; inbounds_spec; outbounds_spec; use_bitwidth_in_spec; use_bitwidth_out_spec]
+               ; Arg.anon_args := [src_n_spec; sc_spec; src_limbwidth_spec; dst_limbwidth_spec]
+               ; Arg.anon_opt_args := []
+               ; Arg.anon_opt_repeated_arg := Some (function_to_synthesize_spec BaseConversion.valid_names) |};
+
+          parse_args opts args
+          := let '((inbounds_multiplier, outbounds_multiplier, inbounds, outbounds, use_bitwidth_in, use_bitwidth_out),
+                   ((str_src_n, src_n), (str_sc, (s, c)), (str_src_limbwidth, src_limbwidth), (str_dst_limbwidth, dst_limbwidth)),
+                   tt,
+                   requests) := args in
+             let show_requests := match requests with nil => "(all)" | _ => String.concat ", " requests end in
+             let to_bool ls := (0 <? List.length ls)%nat in
+             let to_string_opt ls := List.nth_error (List.map (@snd _ _) ls) 0 in
+             let inbounds_multiplier := to_string_opt inbounds_multiplier in
+             let outbounds_multiplier := to_string_opt outbounds_multiplier in
+             let inbounds := to_string_opt inbounds in
+             let outbounds := to_string_opt outbounds in
+             let use_bitwidth_in := to_bool use_bitwidth_in in
+             let use_bitwidth_out := to_bool use_bitwidth_out in
+             let '(str_inbounds_multiplier, inbounds_multiplier) := parse_dirbounds_multiplier "in" (inl inbounds_multiplier) in
+             let '(str_outbounds_multiplier, outbounds_multiplier) := parse_dirbounds_multiplier "out" (inl outbounds_multiplier) in
+             let '(str_inbounds, inbounds) := parse_dirbounds "in" (inl inbounds) use_bitwidth_in in
+             let '(str_outbounds, outbounds) := parse_dirbounds "out" (inl outbounds) use_bitwidth_out in
+             match join_errors
+                     (join_errors
+                        inbounds_multiplier
+                        outbounds_multiplier)
+                     (join_errors
+                        inbounds
+                        outbounds)
+             with
+             | inr errs => inr errs
+             | inl ((inbounds_multiplier, outbounds_multiplier), (inbounds, outbounds))
+               => inl ((str_src_n, str_sc, str_src_limbwidth, str_dst_limbwidth, str_inbounds_multiplier, str_outbounds_multiplier, use_bitwidth_in, use_bitwidth_out, str_inbounds, str_outbounds, show_requests),
+                       (src_n, s, c, src_limbwidth, dst_limbwidth, inbounds_multiplier, outbounds_multiplier, inbounds, outbounds, requests))
              end;
 
-          extract_known_args :=
-            fun '(src_n, s, c, src_limbwidth, dst_limbwidth, machine_wordsize, inbounds_multiplier, outbounds_multiplier, inbounds, outbounds, requests)
-            => machine_wordsize;
-
           show_lines_args :=
-            fun '((str_src_n, str_sc, str_src_limbwidth, str_dst_limbwidth, str_machine_wordsize, str_inbounds_multiplier, str_outbounds_multiplier, use_bitwidth_in, use_bitwidth_out, str_inbounds, str_outbounds, show_requests),
-                  (src_n, s, c, src_limbwidth, dst_limbwidth, machine_wordsize, inbounds_multiplier, outbounds_multiplier, inbounds, outbounds, requests))
+            fun '((str_src_n, str_sc, str_src_limbwidth, str_dst_limbwidth, str_inbounds_multiplier, str_outbounds_multiplier, use_bitwidth_in, use_bitwidth_out, str_inbounds, str_outbounds, show_requests),
+                  (src_n, s, c, src_limbwidth, dst_limbwidth, inbounds_multiplier, outbounds_multiplier, inbounds, outbounds, requests))
             => ["requested operations: " ++ show_requests;
-                  "src_n = " ++ show false src_n ++ " (from """ ++ str_src_n ++ """)";
-                  "s-c = " ++ PowersOfTwo.show_Z false s ++ " - " ++ show_c false c ++ " (from """ ++ str_sc ++ """)";
-                  "src_limbwidth = " ++ show false src_limbwidth ++ " (from """ ++ str_src_limbwidth ++ """)";
-                  "dst_limbwidth = " ++ show false dst_limbwidth ++ " (from """ ++ str_dst_limbwidth ++ """)";
-                  "machine_wordsize = " ++ show false machine_wordsize ++ " (from """ ++ str_machine_wordsize ++ """)";
-                  "inbounds_multiplier = " ++ show false inbounds_multiplier ++ " (from """ ++ str_inbounds_multiplier ++ """)";
-                  "outbounds_multiplier = " ++ show false outbounds_multiplier ++ " (from """ ++ str_outbounds_multiplier ++ """)";
-                  "inbounds = " ++ show false inbounds ++ " (from """ ++ str_inbounds ++ """ and use_bithwidth_in = " ++ show false use_bitwidth_in ++ ")";
-                  "outbounds = " ++ show false outbounds ++ " (from """ ++ str_outbounds ++ """ and use_bithwidth_out = " ++ show false use_bitwidth_out ++ ")"];
-
-          pipeline_usage_string := "src_n s-c src_limbwidth dst_limbwidth machine_wordsize [--inbounds-multipler=inbounds_multiplier] [--outbounds-multiplier=outbounds_multiplier] [--inbounds=inbounds] [--outbounds=outbounds] " ++ optional_options_to_usage [use_bitwidth_in_and_help; use_bitwidth_out_and_help] ++ " [function_to_synthesize*]";
-
-          help_lines := [src_n_help;
-                           src_limbwidth_help;
-                           dst_limbwidth_help;
-                           machine_wordsize_help;
-                           inbounds_multiplier_help;
-                           outbounds_multiplier_help;
-                           to_help use_bitwidth_in_and_help;
-                           to_help use_bitwidth_out_and_help;
-                           inbounds_help;
-                           outbounds_help;
-                           function_to_synthesize_help BaseConversion.valid_names];
+               "src_n = " ++ show false src_n ++ " (from """ ++ str_src_n ++ """)";
+               "s-c = " ++ PowersOfTwo.show_Z false s ++ " - " ++ show_c false c ++ " (from """ ++ str_sc ++ """)";
+               "src_limbwidth = " ++ show false src_limbwidth ++ " (from """ ++ str_src_limbwidth ++ """)";
+               "dst_limbwidth = " ++ show false dst_limbwidth ++ " (from """ ++ str_dst_limbwidth ++ """)";
+               "inbounds_multiplier = " ++ show false inbounds_multiplier ++ " (from """ ++ str_inbounds_multiplier ++ """)";
+               "outbounds_multiplier = " ++ show false outbounds_multiplier ++ " (from """ ++ str_outbounds_multiplier ++ """)";
+               "inbounds = " ++ show false inbounds ++ " (from """ ++ str_inbounds ++ """ and use_bithwidth_in = " ++ show false use_bitwidth_in ++ ")";
+               "outbounds = " ++ show false outbounds ++ " (from """ ++ str_outbounds ++ """ and use_bithwidth_out = " ++ show false use_bitwidth_out ++ ")"];
 
           Synthesize
-          := fun _ opts '(src_n, s, c, src_limbwidth, dst_limbwidth, machine_wordsize, inbounds_multiplier, outbounds_multiplier, inbounds, outbounds, requests) comment_header prefix
+          := fun _ opts '(src_n, s, c, src_limbwidth, dst_limbwidth, inbounds_multiplier, outbounds_multiplier, inbounds, outbounds, requests) comment_header prefix
              => BaseConversion.Synthesize s c src_n src_limbwidth dst_limbwidth machine_wordsize inbounds_multiplier outbounds_multiplier inbounds outbounds comment_header prefix requests
         }.
 
