src/Rewriter/PerfTesting/Core.v
@@ -54,6 +54,7 @@ Local Instance : should_split_mul_opt := false.
 Local Instance : should_split_multiret_opt := false.
 Local Instance : widen_bytes_opt := false.
 Local Instance : widen_carry_opt := false.
+Local Instance : tight_upperbound_fraction_opt := default_tight_upperbound_fraction.
 
 Import API.
 
